A: alloc, read, write, free ok (pt-only)

src/Steel.Array.fsti
@@ -16,8 +16,6 @@ module U = FStar.Universe
 open FStar.Seq
 open Seq.Aux
 
-let perm = option perm
-
 let array_ref (a: Type0) (#n: nat) : Type u#0
   = H.array_ref (U.raise_t a) #n
 
@@ -27,17 +25,47 @@ let null (#a: Type0) (#n: nat)
 let is_null (#a: Type0) (#n: nat)
   = H.is_null #(U.raise_t a) #n
 
+#set-options "--print_implicits"
+
+let perm_ok (#n: nat) = H.perm_ok #n
+
+let raise_val_seq (#a: Type0)
+  (#n: nat)
+  (s: lseq a n)
+  : lseq (U.raise_t a) n
+  =
+  map_seq_len U.raise_val s;
+  map_seq U.raise_val s
+
+let downgrade_val_seq (#a: Type0)
+  (#[@@@smt_fallback] n: nat)
+  (s: lseq (U.raise_t a) n)
+  : lseq a n
+  =
+  map_seq_len U.downgrade_val s;
+  map_seq U.downgrade_val s
+
+let downgrade_raise_val_bij (#a: Type0) (#n: nat) (s: lseq a n)
+  : Lemma
+  (downgrade_val_seq (raise_val_seq s) == s)
+  =
+  admit ();
+  let s' = raise_val_seq s in
+  Classical.forall_intro (map_seq_index U.raise_val s);
+  let s'' = downgrade_val_seq s' in
+  Classical.forall_intro (map_seq_index U.downgrade_val s');
+  ()
+
 let pts_to_sl (#a: Type0)
   (#n: nat)
   (r: array_ref a #n)
   (i1: nat)
-  (i2: nat{i1 < i2 /\ i2 <= n})
-  (p: lseq perm n)
+  (i2: nat{i1 <= i2 /\ i2 <= n})
+  (p: lseq (option perm) n{perm_ok p})
+  (subv: lseq a (i2 - i1))
   =
-  fun (x: lseq a (i2 - i1 + 1)) ->
-    map_seq_len (U.raise_val) x;
-    let x' = map_seq (U.raise_val) x in
-    H.pts_to_sl n r i1 i2 p x'
+  let subv' = raise_val_seq subv in
+  H.pts_to_sl n r i1 i2 p subv'
 
 let raise_val_inj (#a: Type) (x y: a)
   : Lemma
@@ -47,20 +75,15 @@ let raise_val_inj (#a: Type) (x y: a)
   U.downgrade_val_raise_val x;
   U.downgrade_val_raise_val y
 
-let raise_val_seq_inj (#a: Type) (x y: seq a)
+let raise_val_seq_inj (#a: Type) (#n: nat) (x y: lseq a n)
   : Lemma
   (requires
-    map_seq U.raise_val x == map_seq U.raise_val y
+    raise_val_seq x == raise_val_seq y
   )
   (ensures x == y)
   =
-  map_seq_len U.raise_val x;
-  map_seq_len U.raise_val y;
-  let x' = map_seq U.raise_val x in
-  let y' = map_seq U.raise_val y in
-  assert (length x' == length y');
-  assert (length x == length y);
-  let n = Seq.length x in
+  let x' = raise_val_seq x in
+  let y' = raise_val_seq y in
   Classical.forall_intro (map_seq_index U.raise_val x);
   Classical.forall_intro (map_seq_index U.raise_val y);
   assert(forall (i:nat{i < n}).
@@ -74,15 +97,14 @@ let raise_val_seq_inj (#a: Type) (x y: seq a)
   = raise_val_inj (index x i) (index y i)
   in
   Classical.forall_intro aux;
-  Seq.lemma_eq_intro x y;
-  ()
+  Seq.lemma_eq_intro x y
 
 let pts_to_ref_injective (#a: Type0) (#n: nat)
   (r: array_ref a #n)
   (i1: nat)
-  (i2: nat{i1 < i2 /\ i2 <= n})
-  (p1 p2: lseq perm n)
-  (subv1 subv2: lseq a (i2 - i1 + 1))
+  (i2: nat{i1 <= i2 /\ i2 <= n})
+  (p1 p2: (p:lseq (option perm) n{perm_ok p}))
+  (subv1 subv2: lseq a (i2 - i1))
   (m:Mem.mem)
   : Lemma
     (requires Mem.interp (
@@ -90,33 +112,30 @@ let pts_to_ref_injective (#a: Type0) (#n: nat)
       pts_to_sl r i1 i2 p2 subv2) m)
     (ensures subv1 == subv2)
   =
-  map_seq_len U.raise_val subv1;
-  map_seq_len U.raise_val subv2;
-  let subv1' = map_seq U.raise_val subv1 in
-  let subv2' = map_seq U.raise_val subv2 in
+  let subv1' = raise_val_seq subv1 in
+  let subv2' = raise_val_seq subv2 in
   H.pts_to_ref_injective r i1 i2 p1 p2 subv1' subv2' m;
   raise_val_seq_inj subv1 subv2
 
 let pts_to_not_null (#a:Type0) (#n: nat)
   (r: array_ref a #n)
   (i1: nat)
-  (i2: nat{i1 < i2 /\ i2 <= n})
-  (p: lseq perm n)
-  (subv: lseq a (i2 - i1 + 1))
+  (i2: nat{i1 <= i2 /\ i2 <= n})
+  (p: lseq (option perm) n{perm_ok p})
+  (subv: lseq a (i2 - i1))
   (m:Mem.mem)
   : Lemma (requires Mem.interp (pts_to_sl r i1 i2 p subv) m)
           (ensures r =!= null)
   =
-  map_seq_len U.raise_val subv;
-  let subv' = map_seq U.raise_val subv in
+  let subv' = raise_val_seq subv in
   H.pts_to_not_null r i1 i2 p subv' m
 
 let aux_sl (#a: Type0) (#n: nat)
   (r: array_ref a #n)
   (i1: nat)
-  (i2: nat{i1 < i2 /\ i2 <= n})
-  (p: lseq perm n)
-  (subv1 subv2: lseq a (i2 - i1 + 1))
+  (i2: nat{i1 <= i2 /\ i2 <= n})
+  (p: lseq (option perm) n{perm_ok p})
+  (subv1 subv2: lseq a (i2 - i1))
   (m:Mem.mem)
   : Lemma
   (requires
@@ -125,12 +144,10 @@ let aux_sl (#a: Type0) (#n: nat)
   )
   (ensures subv1 == subv2)
   =
-  map_seq_len U.raise_val subv1;
-  map_seq_len U.raise_val subv2;
-  let subv1' : lseq (U.raise_t a) (i2 - i1 + 1)
-    = map_seq U.raise_val subv1 in
-  let subv2' : lseq (U.raise_t a) (i2 - i1 + 1)
-    = map_seq U.raise_val subv2 in
+  let subv1' : lseq (U.raise_t a) (i2 - i1)
+    = raise_val_seq subv1 in
+  let subv2' : lseq (U.raise_t a) (i2 - i1)
+    = raise_val_seq subv2 in
   assert (Mem.interp (
     H.pts_to_sl n r i1 i2 p subv1'
   ) m);
@@ -138,14 +155,13 @@ let aux_sl (#a: Type0) (#n: nat)
     H.pts_to_sl n r i1 i2 p subv2'
   ) m);
   H.aux_sl r i1 i2 p subv1' subv2' m;
-  raise_val_seq_inj subv1 subv2;
-  ()
+  raise_val_seq_inj subv1 subv2
 
 let pts_to_witinv (#a:Type) (#n: nat)
   (r:array_ref a #n)
   (i1: nat)
-  (i2: nat{i1 < i2 /\ i2 < n})
-  (p: lseq perm n)
+  (i2: nat{i1 <= i2 /\ i2 <= n})
+  (p: lseq (option perm) n{perm_ok p})
   : Lemma (Mem.is_witness_invariant (
       pts_to_sl r i1 i2 p
     ))
@@ -159,20 +175,20 @@ let pts_to_witinv (#a:Type) (#n: nat)
 let pts_to (#a: Type) (#n: nat)
   (r: array_ref a #n)
   (i1: nat)
-  (i2: nat{i1 < i2 /\ i2 <= n})
-  ([@@@smt_fallback] p: lseq perm n)
-  ([@@@smt_fallback] subv: lseq a (i2 - i1 + 1))
+  (i2: nat{i1 <= i2 /\ i2 <= n})
+  (p: lseq (option perm) n{perm_ok p})
+  (subv: lseq a (i2 - i1))
   : vprop
   = to_vprop (pts_to_sl r i1 i2 p subv)
 
-let pts_to_injectiv_eq (#a: Type)
+let pts_to_injective_eq (#a: Type)
   (#n: nat)
   (#opened:Mem.inames)
   (r: array_ref a #n)
   (i1: nat)
   (i2: nat{i1 < i2 /\ i2 < n})
-  (p1 p2: lseq perm n)
-  (subv1 subv2: lseq a (i2 - i1 + 1))
+  (p1 p2: (p:lseq (option perm) n{perm_ok p}))
+  (subv1 subv2: lseq a (i2 - i1))
   : SteelGhost unit opened
   (pts_to r i1 i2 p1 subv1 `star`
    pts_to r i1 i2 p2 subv2)
@@ -191,17 +207,102 @@ let pts_to_injectiv_eq (#a: Type)
     (pts_to r i1 i2 p2 subv1)
     (fun _ -> ())
 
-let mk_perm (n: nat) (p: perm)
-  = Seq.create n p
+//let mk_perm n p : lseq (option perm) n = Seq.create n p
 
-let alloc_pt (#a: Type)
+let slu_downgrade (#a: Type0) (#n: nat)
+  (r: array_ref a #n)
+  (i1: nat)
+  (i2: nat{i1 <= i2 /\ i2 <= n})
+  (p: lseq (option perm) n{perm_ok p})
+  (subv: lseq a (i2 - i1))
+  : SteelT unit
+  (H.pts_to r i1 i2 p (raise_val_seq subv))
+  (fun _ -> pts_to r i1 i2 p subv)
+  =
+  rewrite_slprop
+    (H.pts_to r i1 i2 p (raise_val_seq subv))
+    (pts_to r i1 i2 p subv)
+    (fun m -> assert_norm (
+      hp_of (H.pts_to r i1 i2 p (raise_val_seq subv))
+   == hp_of (pts_to r i1 i2 p subv)
+    ))
+
+let slu_raise (#a: Type0) (#n: nat)
+  (r: array_ref a #n)
+  (i1: nat)
+  (i2: nat{i1 <= i2 /\ i2 <= n})
+  (p: lseq (option perm) n{perm_ok p})
+  (subv: lseq a (i2 - i1))
+  : SteelT unit
+  (pts_to r i1 i2 p subv)
+  (fun _ -> H.pts_to r i1 i2 p (raise_val_seq subv))
+  =
+  rewrite_slprop
+    (pts_to r i1 i2 p subv)
+    (H.pts_to r i1 i2 p (raise_val_seq subv))
+    (fun m -> assert_norm (
+      hp_of (H.pts_to r i1 i2 p (raise_val_seq subv))
+   == hp_of (pts_to r i1 i2 p subv)
+    ))
+
+let alloc_pt (#a: Type0)
   (n: nat)
   (v: lseq a n)
   : Steel
   (array_ref a #n)
   emp
-  (fun r -> pts_to r 0 (n-1) (mk_perm n (Some full_perm)) v)
+  (fun r -> pts_to r 0 n (H.full_perm_seq n) v)
   (requires fun _ -> True)
   (ensures fun _ r _ -> not (is_null r))
   =
-  admit ()
+  let r = H.alloc2 n (raise_val_seq v) in
+  slu_downgrade r 0 n (H.full_perm_seq n) v;
+  return r
+
+let read_pt (#a: Type0) (n:nat)
+  (r: array_ref a #n)
+  (i1: nat)
+  (i2: nat{i1 <= i2 /\ i2 <= n})
+  (p: lseq (option perm) n{perm_ok p /\ H.zeroed (i1, i2) p})
+  (#subv: lseq a (i2 - i1))
+  : Steel (lseq a (i2 - i1))
+  (pts_to #a #n r i1 i2 p subv)
+  (fun _ -> pts_to #a #n r i1 i2 p subv)
+  (requires fun _ -> True)
+  (ensures fun _ subv' _ -> subv' == subv)
+  =
+  slu_raise r i1 i2 p subv;
+  let subv' = H.read2 n r i1 i2 p #_ in
+  let subv' = downgrade_val_seq subv' in
+  downgrade_raise_val_bij subv;
+  slu_downgrade r i1 i2 p subv;
+  return subv'
+
+let write_pt (#a: Type0) (n: nat)
+  (r: array_ref a #n)
+  (i1: nat)
+  (i2: nat{i1 <= i2 /\ i2 <= n})
+  (p: lseq (option perm) n{
+    perm_ok p /\ H.zeroed (i1, i2) p /\ H.full_p (i1, i2) p})
+  (subv: lseq a (i2 - i1))
+  (subv_to_write: lseq a (i2 - i1))
+  : SteelT unit
+  (pts_to #a #n r i1 i2 p subv)
+  (fun _ -> pts_to #a #n r i1 i2 p subv_to_write)
+  =
+  slu_raise r i1 i2 p subv;
+  H.write2 n r i1 i2 p
+    (raise_val_seq subv)
+    (raise_val_seq subv_to_write);
+  slu_downgrade r i1 i2 p subv_to_write
+
+let free_pt (#a: Type) (n:nat)
+  (r: array_ref a #n)
+  (p: lseq (option perm) n{p == H.full_perm_seq n})
+  (subv: lseq a n)
+  : SteelT unit
+  (pts_to #a #n r 0 n p subv)
+  (fun _ -> emp)
+  =
+  slu_raise r 0 n p subv;
+  H.free2 n r p (raise_val_seq subv)
